CertiGC/spatial_gcgraph.v
@@ -4,11 +4,11 @@ Require Import VST.msl.shares.
 Require Export VST.msl.wand_frame.
 Require Import RamifyCoq.lib.List_ext.
 Require Import RamifyCoq.msl_ext.log_normalize.
-Require Import RamifyCoq.msl_ext.iter_sepcon.
 Require Import RamifyCoq.msl_ext.ramification_lemmas.
 Require Import RamifyCoq.graph.graph_model.
 Require Import RamifyCoq.CertiGC.GCGraph.
 Require Export RamifyCoq.CertiGC.env_graph_gc.
+Require Import RamifyCoq.msl_ext.iter_sepcon.
 
 Definition vertex_at (sh: share) (p: val) (header: Z) (lst_fields: list val) :=
   data_at sh tuint (Z2val header) (offset_val (- WORD_SIZE) p) *
@@ -750,3 +750,37 @@ Qed.
 
 Lemma isptr_is_pointer_or_integer: forall p, isptr p -> is_pointer_or_integer p.
 Proof. intros. destruct p; try contradiction. exact I. Qed.
+
+Lemma heap_rest_rep_cut: forall (h: heap) i s (H1: 0 <= i < Zlength (spaces h))
+                                (H2: has_space (Znth i (spaces h)) s),
+    space_start (Znth i (spaces h)) <> nullval ->
+    heap_rest_rep h =
+    data_at_ (space_sh (Znth i (spaces h))) (tarray int_or_ptr_type s)
+             (offset_val (WORD_SIZE * used_space (Znth i (spaces h)))
+                         (space_start (Znth i (spaces h)))) *
+    heap_rest_rep (cut_heap h i s H1 H2).
+Proof.
+  intros. unfold heap_rest_rep.
+  pose proof (split3_full_length_list
+                0 i _ _ H1 (Zminus_0_l_reverse (Zlength (spaces h)))).
+  replace (i - 0) with i in H0 by omega. simpl in *.
+  remember (firstn (Z.to_nat i) (spaces h)) as l1.
+  remember (skipn (Z.to_nat (i + 1)) (spaces h)) as l2.
+  assert (Zlength l1 = i). {
+    rewrite Zlength_length by omega. subst l1. apply firstn_length_le.
+    rewrite Zlength_correct in H1. rep_omega. }
+  rewrite H0 at 5. rewrite (upd_Znth_char _ _ _ _ _ H3).
+  rewrite H0 at 1. rewrite !iter_sepcon_app_sepcon. simpl.
+  remember (data_at_ (space_sh (Znth i (spaces h))) (tarray int_or_ptr_type s)
+                     (offset_val (WORD_SIZE * used_space (Znth i (spaces h)))
+                                 (space_start (Znth i (spaces h))))) as P.
+  rewrite (sepcon_comm P), sepcon_assoc. f_equal.
+  rewrite (sepcon_comm _ P), <- sepcon_assoc. f_equal.
+  unfold space_rest_rep. simpl. do 2 rewrite if_false by assumption.
+  red in H2. subst P. remember (Znth i (spaces h)) as sp.
+  rewrite (data_at__tarray_value _ _ _ _ H2). rewrite offset_offset_val.
+  replace (total_space sp - used_space sp - s) with
+      (total_space sp - (used_space sp + s)) by omega.
+  replace (WORD_SIZE * used_space sp + WORD_SIZE * s) with
+      (WORD_SIZE * (used_space sp + s))%Z by rep_omega. reflexivity.
+Qed.
